compiler/dafny/tests/basic/print_tuple.dfy
@@ -1,7 +1,6 @@
 method Main() {
 	print (), "\n";
 	print ("ab"), "\n"; // not a tuple
-	print ("ab", ghost "ab"), "\n";
 	print (1, 2), "\n";
 	print ("ab", 3, true), "\n";
 }
